typ_disjoint, array_group_disjoint

share/pulse/examples/dice/cbor/CDDL.Interpreter.Elab.fst
@@ -228,3 +228,367 @@ and rewrite_group_correct
   | GDef _ _ -> ()
 
 #pop-options
+
+(* Disjointness *)
+
+noeq
+type result (t: Type) =
+| RSuccess of t
+| RFailure of string
+| ROutOfFuel
+
+let destruct_group
+  (#n: name_env_elem)
+  (g: group n)
+: Tot (group n & group n)
+= match g with
+  | GConcat g1 g2 -> (g1, g2)
+  | _ -> (g, GNop)
+
+let maybe_close_array_group_concat
+  (close: bool)
+  (a1 a2: Spec.array_group3 None)
+: Lemma
+  (Spec.array_group3_equiv
+    (Spec.maybe_close_array_group (Spec.array_group3_concat a1 a2) close)
+    (Spec.array_group3_concat a1 (Spec.maybe_close_array_group a2 close))
+  )
+= ()
+
+let array_group_sem_destruct_group
+  (e: sem_env)
+  (g: group NArrayGroup { group_bounded _ e.se_bound g })
+: Lemma
+  (let (g1, g2) = destruct_group g in
+    group_bounded _ e.se_bound g1 /\
+    group_bounded _ e.se_bound g2 /\
+    array_group_sem e g `Spec.array_group3_equiv` (array_group_sem e g1 `Spec.array_group3_concat` array_group_sem e g2)
+  )
+= ()
+
+let maybe_close_array_group_sem_destruct_group
+  (close: bool)
+  (e: sem_env)
+  (g: group NArrayGroup { group_bounded _ e.se_bound g })
+: Lemma
+  (let (g1, g2) = destruct_group g in
+    group_bounded _ e.se_bound g1 /\
+    group_bounded _ e.se_bound g2 /\
+    Spec.maybe_close_array_group (array_group_sem e g) close `Spec.array_group3_equiv`
+      (array_group_sem e g1 `Spec.array_group3_concat` Spec.maybe_close_array_group (array_group_sem e g2) close)
+  )
+  [SMTPat (Spec.maybe_close_array_group (array_group_sem e g) close)]
+= ()
+
+#restart-solver
+let array_group_concat_elem_same_disjoint
+  (close: bool)
+  (t1 t2: Spec.typ)
+  (a1 a2: Spec.array_group3 None)
+: Lemma
+  (requires
+    Spec.typ_equiv t1 t2
+  )
+  (ensures (Spec.array_group3_disjoint (Spec.maybe_close_array_group a1 close) (Spec.maybe_close_array_group a2 close) ==>
+    Spec.array_group3_disjoint
+      (Spec.maybe_close_array_group (Spec.array_group3_concat (Spec.array_group3_item t1) a1) close)
+      (Spec.maybe_close_array_group (Spec.array_group3_concat (Spec.array_group3_item t2) a2) close)
+  ))
+= maybe_close_array_group_concat close (Spec.array_group3_item t1) a1;
+  maybe_close_array_group_concat close (Spec.array_group3_item t1) a2
+
+#push-options "--z3rlimit 128 --query_stats --split_queries always --fuel 4 --ifuel 8"
+
+#restart-solver
+[@@"opaque_to_smt"]
+let rec typ_disjoint
+  (e: ast_env)
+  (fuel: nat)
+  (t1: typ { typ_bounded e.e_sem_env.se_bound t1 })
+  (t2: typ { typ_bounded e.e_sem_env.se_bound t2 })
+: Pure (result unit) // I cannot use `squash` because of unification, yet I want to shortcut disjointness symmetry
+    (requires True)
+    (ensures fun r -> RSuccess? r ==> Spec.typ_disjoint (typ_sem e.e_sem_env t1) (typ_sem e.e_sem_env t2))
+    (decreases fuel)
+= if fuel = 0
+  then ROutOfFuel
+  else let fuel' : nat = fuel - 1 in
+  match t1, t2 with
+  | t2, TDef i
+  | TDef i, t2 ->
+    let s1 = e.e_sem_env.se_env i in
+    let t1' = e.e_env i in
+    typ_disjoint e fuel' t1' t2
+  | TChoice t1l t1r, t2
+  | t2, TChoice t1l t1r ->
+    let rl = typ_disjoint e fuel' t1l t2 in
+    if not (RSuccess? rl)
+    then rl
+    else typ_disjoint e fuel' t1r t2
+  | TTagged tag1 t1', TTagged tag2 t2' ->
+    if tag1 = tag2
+    then typ_disjoint e fuel' t1' t2'
+    else RSuccess ()
+  | TTagged _ _, _
+  | _, TTagged _ _ -> RSuccess ()
+  | TElem EBool, TElem (ELiteral (LSimple v))
+  | TElem (ELiteral (LSimple v)), TElem EBool ->
+    if v = Spec.simple_value_true
+    then RFailure "typ_disjoint: Bool vs. simple_value_true"
+    else if v = Spec.simple_value_false
+    then RFailure "typ_disjoint: Bool vs. simple_value_false"
+    else RSuccess ()
+  | TElem (ELiteral (LString ty _)), TElem EByteString
+  | TElem EByteString, TElem (ELiteral (LString ty _)) ->
+    if ty = CBOR.Spec.cbor_major_type_byte_string
+    then RFailure "typ_disjoint: byte string"
+    else RSuccess ()
+  | TElem (ELiteral (LString ty _)), TElem ETextString
+  | TElem ETextString, TElem (ELiteral (LString ty _)) ->
+    if ty = CBOR.Spec.cbor_major_type_text_string
+    then RFailure "typ_disjoint: text string"
+    else RSuccess ()
+  | TElem e1, TElem e2 ->
+    if e1 = e2
+    then RFailure "typ_disjoint: equal elem"
+    else RSuccess ()
+  | TElem _, _
+  | _, TElem _ -> RSuccess ()
+  | TMap _, TMap _ -> RFailure "typ_disjoint: map: not supported"
+  | TMap _, _
+  | _, TMap _ -> RSuccess ()
+  | TArray a1, TArray a2 ->
+    Spec.array3_close_array_group (array_group_sem e.e_sem_env a1);
+    Spec.array3_close_array_group (array_group_sem e.e_sem_env a2);
+    array_group_disjoint e fuel' true a1 a2
+  | TArray _, _
+  | _, TArray _ -> RSuccess ()
+
+and array_group_disjoint
+  (e: ast_env)
+  (fuel: nat)
+  (close: bool)
+  (a1: group NArrayGroup { group_bounded _ e.e_sem_env.se_bound a1 })
+  (a2: group NArrayGroup { group_bounded _ e.e_sem_env.se_bound a2 })
+: Pure (result unit)
+    (requires True)
+    (ensures fun r ->
+      RSuccess? r ==> Spec.array_group3_disjoint (Spec.maybe_close_array_group (array_group_sem e.e_sem_env a1) close) (Spec.maybe_close_array_group (array_group_sem e.e_sem_env a2) close)
+    )
+    (decreases fuel)
+= let a10 = a1 in
+  let a20 = a2 in
+  if fuel = 0
+  then ROutOfFuel
+  else let fuel' : nat = fuel - 1 in
+  match (a1, destruct_group a1), (a2, destruct_group a2) with
+  | (GAlwaysFalse, _), _
+  | _, (GAlwaysFalse, _) -> RSuccess ()
+  | (GNop, _), (GNop, _) -> RFailure "array_group_disjoint: nop"
+  | (GChoice a1l a1r, _), (a2, _)
+  | (a2, _), (GChoice a1l a1r, _) ->
+    let res1 = array_group_disjoint e fuel' close a1l a2 in
+    if not (RSuccess? res1)
+    then res1
+    else array_group_disjoint e fuel' close a1r a2
+  | (_, (GDef _ n, a1r)), (a2, _)
+  | (a2, _), (_, (GDef _ n, a1r)) ->
+    let a1' = GConcat (e.e_env n) a1r in
+    rewrite_group_correct e.e_sem_env fuel' a1';
+    array_group_disjoint e fuel' close (rewrite_group fuel' _ a1') a2
+  | (a1, (GZeroOrMore g, a1r)), (a2, _)
+  | (a2, _), (a1, (GZeroOrMore g, a1r)) ->
+    assert (
+     Spec.array_group3_disjoint (Spec.maybe_close_array_group (array_group_sem e.e_sem_env a10) close) (Spec.maybe_close_array_group (array_group_sem e.e_sem_env a20) close) <==>
+       Spec.array_group3_disjoint (Spec.maybe_close_array_group (array_group_sem e.e_sem_env a1) close) (Spec.maybe_close_array_group (array_group_sem e.e_sem_env a2) close)
+     );
+     let res1 = array_group_disjoint e fuel' close a1r a2 in
+     if not (RSuccess? res1)
+     then res1
+     else if RSuccess? (array_group_disjoint e fuel' false g a2) // loop-free shortcut, but will miss things like "disjoint? (a* ) (ab)"
+     then RSuccess ()
+     else begin
+       Spec.array_group3_concat_assoc (array_group_sem e.e_sem_env g) (array_group_sem e.e_sem_env (GZeroOrMore g)) (array_group_sem e.e_sem_env a1r);
+       let a1' = GConcat g a1 in
+       rewrite_group_correct e.e_sem_env fuel' a1';
+       array_group_disjoint e fuel' close (rewrite_group fuel' _ a1') a2 // potential source of loops
+     end
+   | (a1, (GOneOrMore g, a1r)), (a2, _)
+   | (a2, _), (a1, (GOneOrMore g, a1r)) ->
+     assert (
+       Spec.array_group3_disjoint (Spec.maybe_close_array_group (array_group_sem e.e_sem_env a10) close) (Spec.maybe_close_array_group (array_group_sem e.e_sem_env a20) close) <==>
+       Spec.array_group3_disjoint (Spec.maybe_close_array_group (array_group_sem e.e_sem_env a1) close) (Spec.maybe_close_array_group (array_group_sem e.e_sem_env a2) close)
+     );
+     let a1' = GConcat (GConcat g (GZeroOrMore g)) a1r in
+     rewrite_group_correct e.e_sem_env fuel' a1';
+     array_group_disjoint e fuel' close (rewrite_group fuel' _ a1') a2 // potential source of loops
+   | (a1, (GZeroOrOne g, a1r)), (a2, _)
+   | (a2, _), (a1, (GZeroOrOne g, a1r)) ->
+     assert (
+       Spec.array_group3_disjoint (Spec.maybe_close_array_group (array_group_sem e.e_sem_env a10) close) (Spec.maybe_close_array_group (array_group_sem e.e_sem_env a20) close) <==>
+       Spec.array_group3_disjoint (Spec.maybe_close_array_group (array_group_sem e.e_sem_env a1) close) (Spec.maybe_close_array_group (array_group_sem e.e_sem_env a2) close)
+     );
+     let res = array_group_disjoint e fuel' close a1r a2 in
+     if not (RSuccess? res)
+     then res
+     else begin
+       let a1' = GConcat g a1r in
+       rewrite_group_correct e.e_sem_env fuel' a1';
+       array_group_disjoint e fuel' close (rewrite_group fuel' _ a1') a2
+     end
+   | (GNop, _), (_, (GArrayElem _ _, _))
+   | (_, (GArrayElem _ _, _)), (GNop, _) ->
+     if close then RSuccess () else RFailure "array_group_disjoint: empty but not close"
+   | (_, (GArrayElem _ a1l, a1r)), (_, (GArrayElem _ a2l, a2r)) ->
+     let res1 = typ_disjoint e fuel' a1l a2l in
+     if RSuccess? res1
+     then res1
+     else if a1l = a2l // TODO: replace with equivalence?
+     then begin
+       array_group_concat_elem_same_disjoint
+         close
+         (typ_sem e.e_sem_env a1l)
+         (typ_sem e.e_sem_env a2l)
+         (array_group_sem e.e_sem_env a1r)
+         (array_group_sem e.e_sem_env a2r);
+       array_group_disjoint e fuel' close a1r a2r
+     end
+     else res1
+   | (_, (GConcat a11 a12, a13)), (a2, _)
+   | (a2, _), (_, (GConcat a11 a12, a13)) ->
+     array_group_disjoint e fuel' close (GConcat a11 (GConcat a12 a13)) a2
+   | _ -> RFailure "array_group_disjoint: array: unsupported pattern"
+
+#pop-options
+
+(*
+
+
+  
+  | TChoice [], _ -> ResultSuccess
+  | TChoice (t1' :: q1'), _ ->
+    let td1 = typ_disjoint e fuel' (TElem t1') t2 in
+    if not (ResultSuccess? td1)
+    then td1
+    else typ_disjoint e fuel' (TChoice q1') t2
+  | _, TChoice _ ->
+    typ_disjoint e fuel' t2 t1
+  | TEscapeHatch _, _
+  | _, TEscapeHatch _ -> ResultFailure "typ_disjoint: TEscapeHatch"
+  | TTag tag1 t1, TTag tag2 t2 ->
+    if tag1 <> tag2
+    then ResultSuccess
+    else typ_disjoint e fuel' (TElem t1) (TElem t2)
+  | _, TTag _ _
+  | TTag _ _, _ -> ResultSuccess
+  | TArray i1, TArray i2 ->
+    Spec.array3_close_array_group (array_group_sem e.e_semenv i1);
+    Spec.array3_close_array_group (array_group_sem e.e_semenv i2);
+    array_group_disjoint e fuel' true i1 i2
+  | TElem (TElemArray i1), TElem (TElemArray i2) ->
+    Spec.array3_close_array_group (array_group_sem e.e_semenv ["", i1]);
+    Spec.array3_close_array_group (array_group_sem e.e_semenv ["", i2]);
+    array_group_disjoint e fuel' true ["", i1] ["", i2]
+  | TArray i1, TElem (TElemArray i2)
+    ->
+    Spec.array3_close_array_group (array_group_sem e.e_semenv i1);
+    Spec.array3_close_array_group (array_group_sem e.e_semenv ["", i2]);
+    array_group_disjoint e fuel' true i1 ["", i2]
+  | TElem (TElemArray i2), TArray i1
+    ->
+    Spec.array3_close_array_group (array_group_sem e.e_semenv i1);
+    Spec.array3_close_array_group (array_group_sem e.e_semenv ["", i2]);
+    array_group_disjoint e fuel' true ["", i2] i1
+  | TArray _, _
+  | _, TArray _ -> ResultSuccess
+  | TElem (TLiteral (TLSimple l1)) , TElem TBool
+  | TElem TBool, TElem (TLiteral (TLSimple l1))
+  -> if l1 = Spec.simple_value_false || l1 = Spec.simple_value_true
+    then ResultFailure "typ_disjoint: TFalse, TBool"
+    else ResultSuccess
+  | TElem (TLiteral (TLString ty1 _)), TElem TByteString
+  | TElem TByteString, TElem (TLiteral (TLString ty1 _))
+  -> if ty1 = cddl_major_type_byte_string
+    then ResultFailure "typ_disjoint: byte_string"
+    else ResultSuccess
+  | TElem (TLiteral (TLString ty1 _)), TElem TTextString
+  | TElem TTextString, TElem (TLiteral (TLString ty1 _))
+  -> if ty1 = cddl_major_type_text_string
+    then ResultFailure "typ_disjoint: byte_string"
+    else ResultSuccess
+  | (TMap _), (TMap _) -> ResultFailure "typ_disjoint: TMap, TMap" // TODO
+  | TMap _, _ | _, TMap _ -> ResultSuccess
+  | TElem e1, TElem e2 ->
+    if e1 <> e2
+    then ResultSuccess
+    else ResultFailure "typ_disjoint: TElem equal"
+
+and array_group_disjoint
+  (e: ast_env)
+  (fuel: nat)
+  (close: bool)
+  (t1: array_group)
+  (t2: array_group)
+: Pure result
+  (requires (
+    array_group_bounded e.e_semenv.se_bound t1 /\
+    array_group_bounded e.e_semenv.se_bound t2
+  ))
+  (ensures (fun b ->
+    array_group_bounded e.e_semenv.se_bound t1 /\
+    array_group_bounded e.e_semenv.se_bound t2 /\
+    (b == ResultSuccess ==> Spec.array_group3_disjoint
+      (Spec.maybe_close_array_group (array_group_sem e.e_semenv t1) close)
+      (Spec.maybe_close_array_group (array_group_sem e.e_semenv t2) close)
+  )))
+  (decreases fuel)
+= if fuel = 0
+  then ResultOutOfFuel
+  else let fuel' : nat = fuel - 1 in
+  match t1, t2 with
+  | (_, TAAtom (TADef i1)) :: q1, _ ->
+    let s1 = e.e_semenv.se_env i1 in
+    if SEArrayGroup? s1
+    then
+      let t1' = e.e_env i1 in
+      array_group_disjoint e fuel' close (t1' `List.Tot.append` q1) t2
+    else ResultSuccess
+  | _, (_, TAAtom (TADef _)) :: _ ->
+    array_group_disjoint e fuel' close t2 t1
+  | (name, TAZeroOrMore t1') :: q, _ ->
+    let res1 = array_group_disjoint e fuel' close q t2 in
+    if not (ResultSuccess? res1)
+    then res1
+    else if ResultSuccess? (array_group_disjoint e fuel' false [name, TAAtom t1'] t2) // loop-free shortcut, but will miss things like "disjoint? (a* ) (ab)"
+    then ResultSuccess
+    else array_group_disjoint e fuel' close ((name, TAAtom t1') :: (name, TAZeroOrMore t1') :: q) t2 // general rule, possible source of loops
+  | _, (_, TAZeroOrMore _) :: _ ->
+    array_group_disjoint e fuel' close t2 t1
+  | (name, TAOneOrMore t1') :: q, _ ->
+    array_group_disjoint e fuel' close ((name, TAAtom t1') :: (name, TAZeroOrMore t1') :: q) t2
+  | _, (_, TAOneOrMore _) :: _ ->
+    array_group_disjoint e fuel' close t2 t1
+  | (name, TAZeroOrOne t1') :: q, _ ->
+    let res1 = array_group_disjoint e fuel' close q t2 in
+    if not (ResultSuccess? res1)
+    then res1
+    else array_group_disjoint e fuel' close ((name, TAAtom t1') :: q) t2
+  | _, (_, TAZeroOrOne _) :: _ ->
+    array_group_disjoint e fuel' close t2 t1
+  | [], [] -> ResultFailure "array_group_disjoint: [], []"
+  | _, [] -> if close then ResultSuccess else ResultFailure "array_group_disjoint: cons, nil, not close"
+  | [], _ ->
+    array_group_disjoint e fuel' close t2 t1
+  | (n1, TAAtom (TAElem t1')) :: q1, (n2, TAAtom (TAElem t2')) :: q2 ->
+    array_group_sem_cons e.e_semenv n1 (TAAtom (TAElem t1')) q1;
+    array_group_sem_cons e.e_semenv n2 (TAAtom (TAElem t2')) q2;
+    if ResultSuccess? (typ_disjoint e fuel' (TElem t1') (TElem t2'))
+    then ResultSuccess
+    else if typ_equiv e fuel' (TElem t1') (TElem t2')
+    then
+      let res = array_group_disjoint e fuel' close q1 q2 in
+      res
+    else ResultFailure "array_group_disjoint: TAElem"
+//  | _ -> false
+
+#pop-options
